Expand the ConstraintIsCompilable machinery to also work with newtypes

Source/DafnyCore/AST/Members/ICodeContext.cs
@@ -170,4 +170,7 @@ public interface RedirectingTypeDecl : ICallable {
   SubsetTypeDecl.WKind WitnessKind { get; }
   Expression/*?*/ Witness { get; }  // non-null iff WitnessKind is Compiled or Ghost
   FreshIdGenerator IdGenerator { get; }
+
+  [FilledInDuringResolution] bool ConstraintIsCompilable { get; set;  }
+  [FilledInDuringResolution] bool CheckedIfConstraintIsCompilable { get; set; } // Set to true lazily by the Resolver when the Resolver fills in "ConstraintIsCompilable".
 }
